Start with monadic reduction

aneris/examples/consensus/paxos_runner.v
@@ -48,6 +48,573 @@ Section runner.
   Context `{!paxosG Σ runner_topo}.
   Context `{anerisG (Paxos_model runner_topo) Σ}.
 
+Inductive nsexpr : Set :=
+| NSMeta : list (string * nsval) → nat → nsexpr
+| NSVal : nsval → nsexpr
+| NSVar : string → nsexpr
+| NSRec : binder → binder → nsexpr → nsexpr
+| NSApp : nsexpr → nsexpr → nsexpr
+| NSUnOp : un_op → nsexpr → nsexpr
+| NSBinOp : bin_op → nsexpr → nsexpr → nsexpr
+| NSIf : nsexpr → nsexpr → nsexpr → nsexpr
+| NSFindFrom : nsexpr → nsexpr → nsexpr → nsexpr
+| NSSubstring : nsexpr → nsexpr → nsexpr → nsexpr
+| NSRand : nsexpr → nsexpr
+| NSPair : nsexpr → nsexpr → nsexpr
+| NSFst : nsexpr → nsexpr
+| NSSnd : nsexpr → nsexpr
+| NSInjL : nsexpr → nsexpr
+| NSInjR : nsexpr → nsexpr
+| NSCase : nsexpr → nsexpr → nsexpr → nsexpr
+| NSFork : nsexpr → nsexpr
+| NSAlloc : option string → nsexpr → nsexpr
+| NSLoad : nsexpr → nsexpr
+| NSStore : nsexpr → nsexpr → nsexpr
+| NSCAS : nsexpr → nsexpr → nsexpr → nsexpr
+| NSMakeAddress : nsexpr → nsexpr → nsexpr
+| NSGetAddressInfo : nsexpr → nsexpr
+| NSNewSocket : nsexpr → nsexpr
+| NSSocketBind : nsexpr → nsexpr → nsexpr
+| NSSendTo : nsexpr → nsexpr → nsexpr → nsexpr
+| NSReceiveFrom : nsexpr → nsexpr
+| NSSetReceiveTimeout : nsexpr → nsexpr → nsexpr → nsexpr
+| NSStart : base_lit → nsexpr → nsexpr
+| NSSetEmpty : nsexpr
+| NSSetAdd : nsexpr → nsexpr → nsexpr
+with nsval : Set :=
+| NSMetaV : nat -> nsval
+  (* HACK: Use HOAS for binders introduced during execution. Replace by a *)
+  (* first order representation. *)
+| NSHoasV : val -> nsval
+| NSLitV : base_lit → nsval
+| NSRecV : binder → binder → nsexpr → nsval
+| NSPairV : nsval → nsval → nsval
+| NSInjLV : nsval → nsval
+| NSInjRV : nsval → nsval
+| NSSetEmptyV : nsval
+| NSSetAddV : nsval.
+
+Inductive nsset : Set :=
+| nsempty.
+
+Inductive NSProp :=
+| NSIsSet : nsset → nsval → NSProp.
+
+Inductive NSFree (A : Type) :=
+| NSPure (a : A)
+| NSForall (k : val → NSFree A)
+| NSAssume (F : NSProp) (k : NSFree A)
+| NSAssert (F : NSProp) (k : NSFree A)
+| NSLater (k : NSFree A).
+
+Notation NSLam x e := (NSRec BAnon x e) (only parsing).
+Notation NSLet x e1 e2 := (NSApp (NSLam x e2) e1) (only parsing).
+Notation NSSeq e1 e2 := (NSLet BAnon e1 e2) (only parsing).
+Notation NSMatch e0 x1 e1 x2 e2 := (NSCase e0 (NSLam x1 e1) (NSLam x2 e2)) (only parsing).
+
+Notation NSubst := (list (string * nsval)).
+Notation Subst := (list (string * val)).
+
+Section Denote.
+
+  Fixpoint substs (s : Subst) (e : expr) {struct s} : expr :=
+    match s with
+    | nil => e
+    | cons (x,v) s' => subst' x v (substs s' e)
+    end.
+
+  Variant meta :=
+  | meta_expr (e : expr)
+  | meta_val  (v : val).
+
+  Context (mmap : list meta).
+
+  Definition ndenote_subst (ndenote_val : nsval -> val) : NSubst -> Subst :=
+    fix ndenote_subst (s : NSubst) {struct s} : Subst :=
+      match s with
+      | nil => nil
+      | cons (x, v) s' => cons (x, ndenote_val v) (ndenote_subst s')
+      end.
+
+  Fixpoint ndenote_expr(e : nsexpr) : expr :=
+    match e with
+    | NSMeta s n => match nth_error mmap n with
+                    | Some (meta_expr e1) => substs (ndenote_subst ndenote_val s) e1
+                    | _                   => #()
+                    end
+    | NSVal v => Val (ndenote_val v)
+    | NSVar x => Var x
+    | NSRec f x e1 => Rec f x (ndenote_expr e1)
+    | NSApp e1 e2 => App (ndenote_expr e1) (ndenote_expr e2)
+    | NSUnOp op e1 => UnOp op (ndenote_expr e1)
+    | NSBinOp op e1 e2 => BinOp op (ndenote_expr e1) (ndenote_expr e2)
+    | NSIf e1 e2 e3 => If (ndenote_expr e1) (ndenote_expr e2) (ndenote_expr e3)
+    | NSFindFrom e1 e2 e3 => FindFrom (ndenote_expr e1) (ndenote_expr e2) (ndenote_expr e3)
+    | NSSubstring e1 e2 e3 => Substring (ndenote_expr e1) (ndenote_expr e2) (ndenote_expr e3)
+    | NSRand e1 => Rand (ndenote_expr e1)
+    | NSPair e1 e2 => Pair (ndenote_expr e1) (ndenote_expr e2)
+    | NSFst e1 => Fst (ndenote_expr e1)
+    | NSSnd e1 => Snd (ndenote_expr e1)
+    | NSInjL e1 => InjL (ndenote_expr e1)
+    | NSInjR e1 => InjR (ndenote_expr e1)
+    | NSCase e1 e2 e3 => Case (ndenote_expr e1) (ndenote_expr e2) (ndenote_expr e3)
+    | NSFork e1 => Fork (ndenote_expr e1)
+    | NSAlloc s e1 => Alloc s (ndenote_expr e1)
+    | NSLoad e1 => Load (ndenote_expr e1)
+    | NSStore e1 e2 => Store (ndenote_expr e1) (ndenote_expr e2)
+    | NSCAS e1 e2 e3 => CAS (ndenote_expr e1) (ndenote_expr e2) (ndenote_expr e3)
+    | NSMakeAddress e1 e2 => MakeAddress (ndenote_expr e1) (ndenote_expr e2)
+    | NSGetAddressInfo e1 => GetAddressInfo (ndenote_expr e1)
+    | NSNewSocket e1 => NewSocket (ndenote_expr e1)
+    | NSSocketBind e1 e2 => SocketBind (ndenote_expr e1) (ndenote_expr e2)
+    | NSSendTo e1 e2 e3 => SendTo (ndenote_expr e1) (ndenote_expr e2) (ndenote_expr e3)
+    | NSReceiveFrom e1 => ReceiveFrom (ndenote_expr e1)
+    | NSSetReceiveTimeout e1 e2 e3 => SetReceiveTimeout (ndenote_expr e1) (ndenote_expr e2) (ndenote_expr e3)
+    | NSStart b e1 => Start b (ndenote_expr e1)
+    | NSSetEmpty => set_empty #()
+    | NSSetAdd e1 e2 => set_add (ndenote_expr e1) (ndenote_expr e2)
+    end
+  with
+  ndenote_val (v : nsval) : val :=
+    match v with
+    | NSMetaV n => match nth_error mmap n with
+                   | Some (meta_val v1) => v1
+                   | _                  => #()
+                   end
+    | NSHoasV v => v
+    | NSLitV v1 => LitV v1
+    | NSRecV f x e => RecV f x (ndenote_expr e)
+    | NSPairV v1 v2 => PairV (ndenote_val v1) (ndenote_val v2)
+    | NSInjLV v1 => InjLV (ndenote_val v1)
+    | NSInjRV v1 => InjRV (ndenote_val v1)
+    | NSSetEmptyV => set_empty
+    | NSSetAddV => set_add
+    end.
+
+  Definition ndenotes (o : option (nsexpr + nsval)) : option (expr + val) :=
+    match o with
+    | Some (inl nse) => Some (inl (ndenote_expr nse))
+    | Some (inr nsv) => Some (inr (ndenote_val nsv))
+    | None           => None
+    end.
+
+  Fixpoint nssubst (x : string) (v : nsval) (e : nsexpr) {struct e} : nsexpr :=
+    match e with
+    | NSMeta s n => NSMeta (cons (x,v) s) n
+    | NSVal v => NSVal v
+    | NSVar y => if decide (x = y) then NSVal v else NSVar y
+    | NSRec f y e0 =>
+        NSRec f y
+          (if decide (and (not (eq (BNamed x) f)) (not (eq (BNamed x) y)))
+           then nssubst x v e0
+           else e0)
+    | NSApp e1 e2 => NSApp (nssubst x v e1) (nssubst x v e2)
+    | NSUnOp op e1 => NSUnOp op (nssubst x v e1)
+    | NSBinOp op e1 e2 => NSBinOp op (nssubst x v e1) (nssubst x v e2)
+    | NSIf e1 e2 e3 => NSIf (nssubst x v e1) (nssubst x v e2) (nssubst x v e3)
+    | NSFindFrom e1 e2 e3 => NSFindFrom (nssubst x v e1) (nssubst x v e2) (nssubst x v e3)
+    | NSSubstring e1 e2 e3 => NSSubstring (nssubst x v e1) (nssubst x v e2) (nssubst x v e3)
+    | NSRand e1 => NSRand (nssubst x v e1)
+    | NSPair e1 e2 => NSPair (nssubst x v e1) (nssubst x v e2)
+    | NSFst e => NSFst (nssubst x v e)
+    | NSSnd e => NSSnd (nssubst x v e)
+    | NSInjL e => NSInjL (nssubst x v e)
+    | NSInjR e => NSInjR (nssubst x v e)
+    | NSCase e1 e2 e3 => NSCase (nssubst x v e1) (nssubst x v e2) (nssubst x v e3)
+    | NSFork e1 => NSFork (nssubst x v e1)
+    | NSAlloc s e1 => NSAlloc s (nssubst x v e1)
+    | NSLoad e => NSLoad (nssubst x v e)
+    | NSStore e1 e2 => NSStore (nssubst x v e1) (nssubst x v e2)
+    | NSCAS e1 e2 e3 => NSCAS (nssubst x v e1) (nssubst x v e2) (nssubst x v e3)
+    | NSMakeAddress e1 e2 => NSMakeAddress (nssubst x v e1) (nssubst x v e2)
+    | NSGetAddressInfo e1 => NSGetAddressInfo (nssubst x v e1)
+    | NSNewSocket e1 => NSNewSocket (nssubst x v e1)
+    | NSSocketBind e1 e2 => NSSocketBind (nssubst x v e1) (nssubst x v e2)
+    | NSSendTo e1 e2 e3 => NSSendTo (nssubst x v e1) (nssubst x v e2) (nssubst x v e3)
+    | NSReceiveFrom e1 => NSReceiveFrom (nssubst x v e1)
+    | NSSetReceiveTimeout e1 e2 e3 => NSSetReceiveTimeout (nssubst x v e1) (nssubst x v e2) (nssubst x v e3)
+    | NSStart b e1 => NSStart b (nssubst x v e1)
+    | NSSetEmpty => NSSetEmpty
+    | NSSetAdd e1 e2 => NSSetAdd (nssubst x v e1) (nssubst x v e2)
+    end.
+
+  Definition nssubst' (mx : binder) (v : nsval) : nsexpr → nsexpr :=
+    match mx with
+    | BAnon => id
+    | BNamed x => nssubst x v
+    end.
+
+  Definition ndenote_set (s : nsset) : gset socket_address :=
+    match s with
+    | nsempty => ∅
+    end.
+
+  Definition ndenote_formula (F : NSProp) : Prop :=
+    match F with
+    | NSIsSet n n0 => is_set (ndenote_set n) (ndenote_val n0)
+    end.
+
+  Fixpoint ndenote_free {R} (m : NSFree R) (Φ : R -> Prop) {struct m} : Prop :=
+    match m with
+    | NSPure _ a => Φ a
+    | NSForall _ k => ∀ v : val, ndenote_free (k v) Φ
+    | NSAssume _ F k => ndenote_formula F → ndenote_free k Φ
+    | NSAssert _ F k => ndenote_formula F ∧ ndenote_free k Φ
+    | NSLater _ k => ndenote_free k Φ
+    end.
+
+End Denote.
+#[global] Arguments ndenote_expr _ _ /.
+#[global] Arguments ndenote_val _ _ /.
+#[global] Arguments ndenotes _ _ /.
+
+    Fixpoint reduce_free_aux {R} (n : nat) :
+      nsexpr → (nsexpr → NSFree R) → (nsval → NSFree R) → NSFree R :=
+      match n with
+      | O   => fun e Ψ Φ => Ψ e
+      | S n => fix go (e : nsexpr) (Ψ : nsexpr → NSFree R)
+                 (Φ : nsval → NSFree R) {struct e} : NSFree R :=
+        match e with
+        | NSMeta s n => Ψ (NSMeta s n)
+        | NSVal v => Φ v
+        | NSPair e1 e2 =>
+            go e2
+              (fun e2' => Ψ (NSPair e1 e2'))
+              (fun v2 =>
+                 go e1
+                   (fun e1' => Ψ (NSPair e1' (NSVal v2)))
+                   (fun v1  => Φ (NSPairV v1 v2)))
+        | NSApp e1 e2 =>
+            go e2
+              (fun e2' => Ψ (NSApp e1 e2'))
+              (fun v2 =>
+                 go e1
+                   (fun e1' => Ψ (NSApp e1' (NSVal v2)))
+                   (fun v1 =>
+                      match v1 with
+                      | NSRecV f x e3 =>
+                          NSLater _ (reduce_free_aux n
+                                    (nssubst' x v2 (nssubst' f (NSRecV f x e3) e3)) Ψ Φ)
+                      | _ => Ψ (NSApp (NSVal v1) (NSVal v2))
+                      end))
+        | NSStore e1 e2 =>
+            go e2
+              (fun e2' => Ψ (NSStore e1 e2'))
+              (fun v2 =>
+                 go e1
+                   (fun e1' => Ψ (NSStore e1' (NSVal v2)))
+                   (fun v1  => Ψ (NSStore (NSVal v1) (NSVal v2))))
+        | NSBinOp op e1 e2 =>
+            go e2
+              (fun e2' => Ψ (NSBinOp op e1 e2'))
+              (fun v2 =>
+                 go e1
+                   (fun e1' => Ψ (NSBinOp op e1' (NSVal v2)))
+                   (fun v1 =>
+                      (* TODO: The concrete reduction of values requires plugging *)
+                      (*                  *)
+                      (* match bin_op_eval op (ndenote_val v1) (ndenote_val v2) with *)
+                      (* | Some v => Φ (NSMetaV v) (S nsteps) *)
+                      (* | None => Ψ (NSBinOp op (NSVal v1) (NSVal v2)) nsteps *)
+                      (* end *)
+                      Ψ (NSBinOp op (NSVal v1) (NSVal v2))))
+        | NSMatch e0 x1 e1 x2 e2 =>
+            go e0
+              (fun e0' => Ψ (NSMatch e0' x1 e1 x2 e2))
+              (fun v0 =>
+                 match v0 with
+                 | NSInjLV v => NSLater _ (reduce_free_aux n (nssubst' x1 v e1) Ψ Φ)
+                 | NSInjRV v => NSLater _ (reduce_free_aux n (nssubst' x2 v e2) Ψ Φ)
+                 | _         => Ψ (NSMatch (NSVal v0) x1 e1 x2 e2)
+                 end)
+        | NSSnd (NSVal (NSPairV v1 v2)) => NSLater _ (Φ v2)
+        | NSRec f x e => NSLater _ (Φ (NSRecV f x e))
+        | NSMakeAddress (NSVal (NSLitV (LitString s))) (NSVal (NSLitV (LitInt p))) =>
+            NSLater _ (Φ (NSLitV (LitSocketAddress (SocketAddressInet s (Z.to_pos p)))))
+        | NSSetEmpty => NSLater _ (NSForall _ (fun v => NSAssume _ (NSIsSet nsempty (NSHoasV v)) (Φ (NSHoasV v))))
+        (* | NSSetAdd e1 e2 => *)
+        (*     go e2 *)
+        (*       (fun e2' => Ψ (NSSetAdd e1 e2')) *)
+        (*       (fun v2 => *)
+        (*          go e1 *)
+        (*            (fun e1' => Ψ (NSSetAdd e1' (NSVal v2))) *)
+        (*            (fun v1 => *)
+        (*               NSAssert (NSIsSet *)
+        (*               Ψ (NSSetAdd (NSVal v1) (NSVal v2))))) *)
+        (*               (* match v1 with *) *)
+        (*               (* | NSRecV f x e3 => *) *)
+        (*               (*     NSLater _ (reduce_free_aux n *) *)
+        (*               (*                 (nssubst' x v2 (nssubst' f (NSRecV f x e3) e3)) Ψ Φ) *) *)
+        (*               (* | _ => Ψ (NSApp (NSVal v1) (NSVal v2)) *) *)
+        (*               (* end)) *) *)
+
+        | _ => Ψ e
+        end
+      end.
+
+    Definition reduce_free (e : nsexpr) : NSFree (nsexpr + nsval) :=
+      reduce_free_aux 10 e (fun e => NSPure _ (inl e)) (fun v => NSPure _ (inr v)).
+    #[global] Arguments reduce_free e /.
+
+    Lemma tac_wp_reduce_free_sound (Δ : environments.envs (iPropI Σ)) E
+      (ip : ip_address) (mmap : list meta) (e : nsexpr) (Φ : val → iProp Σ) :
+      forall m,
+      reduce_free e = m ->
+      ndenote_free mmap m
+        (fun ev =>
+           match ev with
+           | inl e => environments.envs_entails Δ (aneris_wp ip E (ndenote_expr mmap e) Φ)
+           | inr v => environments.envs_entails Δ (▷ Φ (ndenote_val mmap v))
+           end) →
+      environments.envs_entails Δ (aneris_wp ip E (ndenote_expr mmap e) Φ).
+    Proof. Admitted.
+
+    Ltac tac_wp_in_list x xs :=
+      match xs with
+      | @nil _         => false
+      | @cons _ x _    => true
+      | @cons _ _ ?xs' => tac_wp_in_list x xs'
+      end.
+
+    Ltac tac_wp_add_to_mmap m mmap :=
+      let b := tac_wp_in_list m mmap in
+      match b with
+      | true => mmap
+      | false => constr:(@cons meta m mmap)
+      end.
+
+Ltac tac_wp_mk_map_expr
+  mmap0 (* : list meta *)
+  e0    (* : expr *)
+  tac0  (* : list meta -> r *)
+        (* : r *)
+  :=
+  let rec tac_wp_mk_map_expr mmap e tac :=
+    (* idtac "tac_wp_mk_map_expr" mmap e; *)
+    lazymatch e with
+    | Val ?v =>
+        tac_wp_mk_map_val mmap v tac
+    | Var ?x =>
+        (* TODO: We do not allow meta-variables inside strings,
+           so should we check if x is ground? *)
+        tac mmap
+    | Rec ?b1 ?b2 ?e1 =>
+        tac_wp_mk_map_expr mmap e1 tac
+    | App ?e1 ?e2 =>
+        tac_wp_mk_map_expr mmap e1 ltac:(fun mmap1 =>
+        tac_wp_mk_map_expr mmap1 e2 tac)
+    | UnOp ?op ?e1 =>
+        tac_wp_mk_map_expr mmap e1 tac
+    | BinOp ?op ?e1 ?e2 =>
+        tac_wp_mk_map_expr mmap e1 ltac:(fun mmap1 =>
+        tac_wp_mk_map_expr mmap1 e2 tac)
+    | If ?e1 ?e2 ?e3 =>
+        tac_wp_mk_map_expr mmap e1 ltac:(fun mmap1 =>
+        tac_wp_mk_map_expr mmap1 e2 ltac:(fun mmap2 =>
+        tac_wp_mk_map_expr mmap2 e3 tac))
+    | FindFrom ?e1 ?e2 ?e3 =>
+        tac_wp_mk_map_expr mmap e1 ltac:(fun mmap1 =>
+        tac_wp_mk_map_expr mmap1 e2 ltac:(fun mmap2 =>
+        tac_wp_mk_map_expr mmap2 e3 tac))
+    | Substring ?e1 ?e2 ?e3 =>
+        tac_wp_mk_map_expr mmap e1 ltac:(fun mmap1 =>
+        tac_wp_mk_map_expr mmap1 e2 ltac:(fun mmap2 =>
+        tac_wp_mk_map_expr mmap2 e3 tac))
+    | Rand ?e1 =>
+        tac_wp_mk_map_expr mmap e1 tac
+    | Pair ?e1 ?e2 =>
+        tac_wp_mk_map_expr mmap e1 ltac:(fun mmap1 =>
+        tac_wp_mk_map_expr mmap1 e2 tac)
+    | Fst ?e1 =>
+        tac_wp_mk_map_expr mmap e1 tac
+    | Snd ?e1 =>
+        tac_wp_mk_map_expr mmap e1 tac
+    | InjL ?e1 =>
+        tac_wp_mk_map_expr mmap e1 tac
+    | InjR ?e1 =>
+        tac_wp_mk_map_expr mmap e1 tac
+    | Case ?e1 ?e2 ?e3 =>
+        tac_wp_mk_map_expr mmap e1 ltac:(fun mmap1 =>
+        tac_wp_mk_map_expr mmap1 e2 ltac:(fun mmap2 =>
+        tac_wp_mk_map_expr mmap2 e3 tac))
+    | Alloc ?s ?e1 =>
+        tac_wp_mk_map_expr mmap e1 tac
+    | MakeAddress ?e1 ?e2 =>
+        tac_wp_mk_map_expr mmap e1 ltac:(fun mmap1 =>
+        tac_wp_mk_map_expr mmap1 e2 tac)
+    | Start ?b ?e1 =>
+        tac_wp_mk_map_expr mmap e1 tac
+    | _      =>
+        (* idtac "tac_wp_mk_map_expr.default.beforeAddToMap" mmap; *)
+        let mmap' := tac_wp_add_to_mmap constr:(meta_expr e) mmap in
+        (* idtac "tac_wp_mk_map_expr.default.afterAddToMap" mmap'; *)
+        tac mmap'
+    end
+  with tac_wp_mk_map_val mmap v tac :=
+    lazymatch v with
+    | LitV ?b =>
+        (* TODO: We do not allow meta-variables inside base_lits,
+           so should we check if b is ground? *)
+        tac mmap
+    | RecV ?b1 ?b2 ?e1 =>
+        tac_wp_mk_map_expr mmap e1 tac
+    | PairV ?v1 ?v2 =>
+        tac_wp_mk_map_val mmap v1 ltac:(fun mmap1 =>
+        tac_wp_mk_map_val mmap1 v2 tac)
+    | InjLV ?v1 =>
+        tac_wp_mk_map_val mmap v1 tac
+    | InjRV ?v1 =>
+        tac_wp_mk_map_val mmap v1 tac
+    | set_empty =>
+        tac mmap
+    | set_add =>
+        tac mmap
+    | _ =>
+        let mmap' := tac_wp_add_to_mmap constr:(meta_val v) mmap in
+        tac mmap'
+    end
+  in tac_wp_mk_map_expr mmap0 e0 tac0.
+
+Ltac tac_wp_map_lookup
+  (* forall a. *)
+  x  (* : a *)
+  xs (* : list a *)
+     (* : nat *)
+  := lazymatch xs with
+     | @cons _ x _    => O
+     | @cons _ _ ?xs' =>
+         let n := tac_wp_map_lookup x xs' in
+         constr:(S n)
+     end.
+
+Ltac tac_wp_reify_expr mmap e0 :=
+  let rec tac_wp_reify_expr e :=
+    lazymatch e with
+    | App (Val set_empty) (Val (LitV LitUnit)) =>
+        constr:(NSSetEmpty)
+    | Val ?v =>
+        let nsv := tac_wp_reify_val v in
+        constr:(NSVal nsv)
+    | Var ?x =>
+        constr:(NSVar x)
+    | Rec ?b1 ?b2 ?e1 =>
+        let nse1 := tac_wp_reify_expr e1 in
+        constr:(NSRec b1 b2 nse1)
+    | App ?e1 ?e2 =>
+        let nse1 := tac_wp_reify_expr e1 in
+        let nse2 := tac_wp_reify_expr e2 in
+        constr:(NSApp nse1 nse2)
+    | UnOp ?op ?e1 =>
+        let nse1 := tac_wp_reify_expr e1 in
+        constr:(NSUnOp op nse1)
+    | BinOp ?op ?e1 ?e2 =>
+        let nse1 := tac_wp_reify_expr e1 in
+        let nse2 := tac_wp_reify_expr e2 in
+        constr:(NSBinOp op nse1 nse2)
+    | If ?e1 ?e2 ?e3 =>
+        let nse1 := tac_wp_reify_expr e1 in
+        let nse2 := tac_wp_reify_expr e2 in
+        let nse3 := tac_wp_reify_expr e3 in
+        constr:(NSIf nse1 nse2 nse3)
+    | FindFrom ?e1 ?e2 ?e3 =>
+        let nse1 := tac_wp_reify_expr e1 in
+        let nse2 := tac_wp_reify_expr e2 in
+        let nse3 := tac_wp_reify_expr e3 in
+        constr:(NSFindFrom nse1 nse2 nse3)
+    | Substring ?e1 ?e2 ?e3 =>
+        let nse1 := tac_wp_reify_expr e1 in
+        let nse2 := tac_wp_reify_expr e2 in
+        let nse3 := tac_wp_reify_expr e3 in
+        constr:(NSSubstring nse1 nse2 nse3)
+    | Rand ?e1 =>
+        let nse1 := tac_wp_reify_expr e1 in
+        constr:(NSRand op nse1)
+    | Pair ?e1 ?e2 =>
+        let nse1 := tac_wp_reify_expr e1 in
+        let nse2 := tac_wp_reify_expr e2 in
+        constr:(NSPair nse1 nse2)
+    | Fst ?e1 =>
+        let nse1 := tac_wp_reify_expr e1 in
+        constr:(NSFst nse1)
+    | Snd ?e1 =>
+        let nse1 := tac_wp_reify_expr e1 in
+        constr:(NSSnd nse1)
+    | InjL ?e1 =>
+        let nse1 := tac_wp_reify_expr e1 in
+        constr:(NSInjL nse1)
+    | InjR ?e1 =>
+        let nse1 := tac_wp_reify_expr e1 in
+        constr:(NSInjR nse1)
+    | Case ?e1 ?e2 ?e3 =>
+        let nse1 := tac_wp_reify_expr e1 in
+        let nse2 := tac_wp_reify_expr e2 in
+        let nse3 := tac_wp_reify_expr e3 in
+        constr:(NSCase nse1 nse2 nse3)
+    | Alloc ?s ?e1 =>
+        let nse1 := tac_wp_reify_expr e1 in
+        constr:(NSAlloc s nse1)
+    | MakeAddress ?e1 ?e2 =>
+        let nse1 := tac_wp_reify_expr e1 in
+        let nse2 := tac_wp_reify_expr e2 in
+        constr:(NSMakeAddress nse1 nse2)
+    | Start ?b ?e1 =>
+        let nse1 := tac_wp_reify_expr e1 in
+        constr:(NSStart b nse1)
+    | _ =>
+        let n := tac_wp_map_lookup constr:(meta_expr e) mmap in
+        constr:(NSMeta (@nil (string * nsval)) n)
+    end
+  with tac_wp_reify_val v :=
+    lazymatch v with
+    | LitV ?b =>
+        constr:(NSLitV b)
+    | RecV ?b1 ?b2 ?e1 =>
+        let nse1 := tac_wp_reify_expr e1 in
+        constr:(NSRecV b1 b2 nse1)
+    | PairV ?v1 ?v2 =>
+        let nsv1 := tac_wp_reify_val v1 in
+        let nsv2 := tac_wp_reify_val v2 in
+        constr:(NSPairV nsv1 nsv2)
+    | InjLV ?v1 =>
+        let nsv1 := tac_wp_reify_val v1 in
+        constr:(NSInjLV nsv1)
+    | InjRV ?v1 =>
+        let nsv1 := tac_wp_reify_val v1 in
+        constr:(NSInjRV nsv1)
+    | set_empty =>
+        constr:(NSSetEmptyV)
+    | set_add =>
+        constr:(NSSetAddV)
+    | _ =>
+        let n := tac_wp_map_lookup constr:(meta_val v) mmap in
+        constr:(NSMetaV  n)
+    end
+  in tac_wp_reify_expr e0.
+
+Ltac tac_wp_reify :=
+  match goal with
+  |- environments.envs_entails ?E (aneris_wp ?ip ?m ?e ?Φ) =>
+      (* Simplify to reduce some calls to [inject] like [Inject_expr]. *)
+      let e := eval simpl in e in
+      tac_wp_mk_map_expr (@nil meta) e
+        ltac:(fun mmap =>
+                let e' := tac_wp_reify_expr mmap e in
+                change (environments.envs_entails E
+                          (aneris_wp ip m (ndenote_expr mmap e') Φ)))
+  end.
+
+Ltac wp_free_pures :=
+  iStartProof;
+  try
+    (tac_wp_reify;
+     (* eapply because of e' *)
+     simple eapply tac_wp_reduce_free_sound;
+     [ (* reduce = .. *)
+       vm_compute; reflexivity
+     | (* ndenote_free *)
+       simpl
+     ]).
+
   Lemma runner_spec :
     {{{ inv paxosN paxos_inv ∗
         ([∗ set] a ∈ acceptors, a ⤇ acceptor_si) ∗
@@ -66,7 +633,7 @@ Section runner.
     iIntros (Φ) "(#Hinv & #Has_si & #Hps_si & #Hls_si & #Hc_si &
                   Hls & Hch & Hips & Hfrags & Hpend0 & Hpend1) HΦ".
     rewrite /runner.
-    do 8 (wp_makeaddress; wp_let). (* ~1.6s *)
+    (* do 8 (wp_makeaddress; wp_let). (* ~1.6s *) *)
     (* nsreify. *)
     (* simple eapply reduce_sound. *)
     (* vm_compute. *)
@@ -75,13 +642,17 @@ Section runner.
     (* Time swp_pures.  (* 0.27-0.29s *) *)
     (* Time nswp_pures. (* 0.23-0.26s *) *)
     (* Time nswp_pures'. (* 0.013 - 0.016s *) *)
-    wp_apply (wp_set_empty socket_address); [done|]; iIntros (??).
+
+    Time wp_pures.
+    Time wp_free_pures; intros ? ?.
+    (* Time wp_apply (wp_set_empty socket_address); [done|]; iIntros (??). *)
     wp_apply (wp_set_add with "[//]"); iIntros (??).
     wp_apply (wp_set_add with "[//]"); iIntros (??).
     wp_apply (wp_set_add with "[//]"); iIntros (? Has).
     rewrite union_empty_r_L union_assoc_L in Has.
     wp_let.
-    wp_apply (wp_set_empty socket_address); [done|]; iIntros (??).
+    Time wp_free_pures; intros ? ?.
+    (* Time wp_apply (wp_set_empty socket_address); [done|]; iIntros (??). *)
     wp_apply (wp_set_add with "[//]"); iIntros (??).
     wp_apply (wp_set_add with "[//]"); iIntros (? Hls).
     rewrite union_empty_r_L in Hls.
